<?xml version="1.0"?>
<rdf:RDF xmlns="http://purl.obolibrary.org/obo/slso/components/slso_environments.owl#"
     xml:base="http://purl.obolibrary.org/obo/slso/components/slso_environments.owl"
     xmlns:obo="http://purl.obolibrary.org/obo/"
     xmlns:owl="http://www.w3.org/2002/07/owl#"
     xmlns:rdf="http://www.w3.org/1999/02/22-rdf-syntax-ns#"
     xmlns:xml="http://www.w3.org/XML/1998/namespace"
     xmlns:xsd="http://www.w3.org/2001/XMLSchema#"
     xmlns:rdfs="http://www.w3.org/2000/01/rdf-schema#"
     xmlns:oboInOwl="http://www.geneontology.org/formats/oboInOwl#">
    <owl:Ontology rdf:about="http://purl.obolibrary.org/obo/slso/components/slso_environments.owl"/>
    


    <!-- 
    ///////////////////////////////////////////////////////////////////////////////////////
    //
    // Annotation properties
    //
    ///////////////////////////////////////////////////////////////////////////////////////
     -->

    


    <!-- http://purl.obolibrary.org/obo/IAO_0000115 -->

    <owl:AnnotationProperty rdf:about="http://purl.obolibrary.org/obo/IAO_0000115"/>
    


    <!-- http://purl.obolibrary.org/obo/IAO_0000116 -->

    <owl:AnnotationProperty rdf:about="http://purl.obolibrary.org/obo/IAO_0000116"/>
    


    <!-- http://purl.obolibrary.org/obo/IAO_0000119 -->

    <owl:AnnotationProperty rdf:about="http://purl.obolibrary.org/obo/IAO_0000119"/>
    


    <!-- http://www.geneontology.org/formats/oboInOwl#hasExactSynonym -->

    <owl:AnnotationProperty rdf:about="http://www.geneontology.org/formats/oboInOwl#hasExactSynonym"/>
    


    <!-- 
    ///////////////////////////////////////////////////////////////////////////////////////
    //
    // Classes
    //
    ///////////////////////////////////////////////////////////////////////////////////////
     -->

    


    <!-- http://purl.obolibrary.org/obo/ENVO_00000469 -->

    <owl:Class rdf:about="http://purl.obolibrary.org/obo/ENVO_00000469"/>
    


    <!-- http://purl.obolibrary.org/obo/ENVO_00003919 -->

    <owl:Class rdf:about="http://purl.obolibrary.org/obo/ENVO_00003919">
        <rdfs:label>research station</rdfs:label>
    </owl:Class>
    


    <!-- http://purl.obolibrary.org/obo/ENVO_01000254 -->

    <owl:Class rdf:about="http://purl.obolibrary.org/obo/ENVO_01000254"/>
    


    <!-- http://purl.obolibrary.org/obo/ENVO_01001406 -->

    <owl:Class rdf:about="http://purl.obolibrary.org/obo/ENVO_01001406">
        <rdfs:label>laboratory facility</rdfs:label>
    </owl:Class>
    


    <!-- http://purl.obolibrary.org/obo/RBO_00000016 -->

    <owl:Class rdf:about="http://purl.obolibrary.org/obo/RBO_00000016"/>
    


    <!-- http://purl.obolibrary.org/obo/SLSO_0000051 -->

    <owl:Class rdf:about="http://purl.obolibrary.org/obo/SLSO_0000051"/>
    


    <!-- http://purl.obolibrary.org/obo/SLSO_1100010 -->

    <owl:Class rdf:about="http://purl.obolibrary.org/obo/SLSO_1100010">
        <rdfs:subClassOf rdf:resource="http://purl.obolibrary.org/obo/ENVO_01000254"/>
        <rdfs:label>space environment</rdfs:label>
    </owl:Class>
    


    <!-- http://purl.obolibrary.org/obo/SLSO_1100011 -->

    <owl:Class rdf:about="http://purl.obolibrary.org/obo/SLSO_1100011">
        <rdfs:subClassOf rdf:resource="http://purl.obolibrary.org/obo/SLSO_1100010"/>
        <obo:IAO_0000115>The region of space between the Earth and the Moon</obo:IAO_0000115>
        <rdfs:label>cis-lunar space environment</rdfs:label>
        <owl:deprecated rdf:datatype="http://www.w3.org/2001/XMLSchema#boolean">true</owl:deprecated>
    </owl:Class>
    


    <!-- http://purl.obolibrary.org/obo/SLSO_1100012 -->

    <owl:Class rdf:about="http://purl.obolibrary.org/obo/SLSO_1100012">
        <rdfs:subClassOf rdf:resource="http://purl.obolibrary.org/obo/SLSO_1100010"/>
        <obo:IAO_0000115>The region of space between the Earth and Mars</obo:IAO_0000115>
        <rdfs:label>cis-mars space environment</rdfs:label>
        <owl:deprecated rdf:datatype="http://www.w3.org/2001/XMLSchema#boolean">true</owl:deprecated>
    </owl:Class>
    


    <!-- http://purl.obolibrary.org/obo/SLSO_1100013 -->

    <owl:Class rdf:about="http://purl.obolibrary.org/obo/SLSO_1100013">
        <rdfs:subClassOf rdf:resource="http://purl.obolibrary.org/obo/SLSO_1100010"/>
        <obo:IAO_0000115>The regions of the solar system where physical and biological phenomena are relatively unaffected by the physical properties of planets and their moons (e.g. by their gravity, atmospheres, magnetic fields, or albedo radiation) compared to the influence of the Sun (e.g. through its gravitational pull, solar wind, magnetic field, and electromagnetic radiation).</obo:IAO_0000115>
        <oboInOwl:hasExactSynonym>interplanetary space</oboInOwl:hasExactSynonym>
        <rdfs:label>interplanetary space environment</rdfs:label>
    </owl:Class>
    


    <!-- http://purl.obolibrary.org/obo/SLSO_1100014 -->

    <owl:Class rdf:about="http://purl.obolibrary.org/obo/SLSO_1100014">
        <rdfs:subClassOf rdf:resource="http://purl.obolibrary.org/obo/SLSO_1100010"/>
        <obo:IAO_0000115>A region of space defined by a regular, repeating path of a specified object about Earth&apos;s moon</obo:IAO_0000115>
        <rdfs:label>lunar orbit</rdfs:label>
    </owl:Class>
    


    <!-- http://purl.obolibrary.org/obo/SLSO_1100015 -->

    <owl:Class rdf:about="http://purl.obolibrary.org/obo/SLSO_1100015">
        <rdfs:subClassOf rdf:resource="http://purl.obolibrary.org/obo/SLSO_1100010"/>
        <obo:IAO_0000115>The area of the lunar landmass exposed to space</obo:IAO_0000115>
        <rdfs:label>lunar surface</rdfs:label>
    </owl:Class>
    


    <!-- http://purl.obolibrary.org/obo/SLSO_1100016 -->

    <owl:Class rdf:about="http://purl.obolibrary.org/obo/SLSO_1100016">
        <rdfs:subClassOf rdf:resource="http://purl.obolibrary.org/obo/SLSO_1100010"/>
        <obo:IAO_0000115>A region of space defined by a regular, repeating path of a specified object about Mars</obo:IAO_0000115>
        <obo:IAO_0000116>mars orbit is distinct from mars&apos; orbit, the latter of which refers to the orbit of the planet around the sun. The planet name can function as an adjective, meaning an orbit related to or associated with Mars. For example, a &quot;Mars orbit&quot; could be the path of a spacecraft around the planet. &quot;Mars&apos; orbit&quot; (with an apostrophe) uses the possessive form of the noun &quot;Mars&quot; to indicate ownership or association. It specifically refers to the natural path and characteristics of the path of the planet Mars&apos; around the Sun.  
Example of use: The Mars Science Laboratory entered Mars orbit prior to deployment of the landing system containing the Curiosity Rover.</obo:IAO_0000116>
        <oboInOwl:hasExactSynonym>martian orbit</oboInOwl:hasExactSynonym>
        <rdfs:label>mars orbit</rdfs:label>
    </owl:Class>
    


    <!-- http://purl.obolibrary.org/obo/SLSO_1100017 -->

    <owl:Class rdf:about="http://purl.obolibrary.org/obo/SLSO_1100017">
        <rdfs:subClassOf rdf:resource="http://purl.obolibrary.org/obo/SLSO_1100010"/>
        <obo:IAO_0000115>The area of the Mars landmass exposed to the Martian atmosphere</obo:IAO_0000115>
        <oboInOwl:hasExactSynonym>martian surface</oboInOwl:hasExactSynonym>
        <rdfs:label>mars surface</rdfs:label>
    </owl:Class>
    


    <!-- http://purl.obolibrary.org/obo/SLSO_1100018 -->

    <owl:Class rdf:about="http://purl.obolibrary.org/obo/SLSO_1100018">
        <rdfs:subClassOf rdf:resource="http://purl.obolibrary.org/obo/SLSO_1100010"/>
        <obo:IAO_0000115>The outermost solid or liquid area of a planet</obo:IAO_0000115>
        <rdfs:label>planet surface</rdfs:label>
    </owl:Class>
    


    <!-- http://purl.obolibrary.org/obo/SLSO_1100019 -->

    <owl:Class rdf:about="http://purl.obolibrary.org/obo/SLSO_1100019">
        <rdfs:subClassOf rdf:resource="http://purl.obolibrary.org/obo/RBO_00000016"/>
        <rdfs:subClassOf rdf:resource="http://purl.obolibrary.org/obo/SLSO_1100010"/>
        <obo:IAO_0000115>A radiation environment outside a commonly defined boundary marking the beginning of space (frequently the Karman line).</obo:IAO_0000115>
        <rdfs:label>space radiation environment</rdfs:label>
    </owl:Class>
    


    <!-- http://purl.obolibrary.org/obo/SLSO_1100020 -->

    <owl:Class rdf:about="http://purl.obolibrary.org/obo/SLSO_1100020">
        <rdfs:subClassOf rdf:resource="http://purl.obolibrary.org/obo/SLSO_1100019"/>
        <obo:IAO_0000115>The natural radiation environment of a region of a cis-lunar space environment</obo:IAO_0000115>
        <rdfs:label>cis-lunar space radiation environment</rdfs:label>
        <owl:deprecated rdf:datatype="http://www.w3.org/2001/XMLSchema#boolean">true</owl:deprecated>
    </owl:Class>
    


    <!-- http://purl.obolibrary.org/obo/SLSO_1100021 -->

    <owl:Class rdf:about="http://purl.obolibrary.org/obo/SLSO_1100021">
        <rdfs:subClassOf rdf:resource="http://purl.obolibrary.org/obo/SLSO_1100019"/>
        <obo:IAO_0000115>The natural radiation environment of a region of a cis-mars space environment</obo:IAO_0000115>
        <rdfs:label>cis-mars space radiation environment</rdfs:label>
        <owl:deprecated rdf:datatype="http://www.w3.org/2001/XMLSchema#boolean">true</owl:deprecated>
    </owl:Class>
    


    <!-- http://purl.obolibrary.org/obo/SLSO_1100022 -->

    <owl:Class rdf:about="http://purl.obolibrary.org/obo/SLSO_1100022">
        <rdfs:subClassOf rdf:resource="http://purl.obolibrary.org/obo/SLSO_1100019"/>
        <obo:IAO_0000115>The natural radiation environment of a region of interplanetary space</obo:IAO_0000115>
        <oboInOwl:hasExactSynonym>free space radiation environment</oboInOwl:hasExactSynonym>
        <rdfs:label>interplanetary space radiation environment</rdfs:label>
    </owl:Class>
    


    <!-- http://purl.obolibrary.org/obo/SLSO_1100023 -->

    <owl:Class rdf:about="http://purl.obolibrary.org/obo/SLSO_1100023">
        <rdfs:subClassOf rdf:resource="http://purl.obolibrary.org/obo/SLSO_1100031"/>
        <obo:IAO_0000115>The natural radiation environment in lunar orbit. Contributions to the lunar orbit radiation environment include: free space radiation, partially shielded by the body of the Moon; albedo radiation produced by interactions of free space radiation with the lunar crust; and, particles produced by decays of radioactive elements in the lunar crust.</obo:IAO_0000115>
        <rdfs:label>lunar orbit radiation environment</rdfs:label>
    </owl:Class>
    


    <!-- http://purl.obolibrary.org/obo/SLSO_1100024 -->

    <owl:Class rdf:about="http://purl.obolibrary.org/obo/SLSO_1100024">
        <rdfs:subClassOf rdf:resource="http://purl.obolibrary.org/obo/SLSO_1100029"/>
        <rdfs:subClassOf rdf:resource="http://purl.obolibrary.org/obo/SLSO_1100031"/>
        <obo:IAO_0000115>The natural radiation environment on or adjacent to the surface of the moon. Contributions to the lunar surface radiation environment include: free space radiation, partially shielded by the body of the Moon; albedo radiation produced by interactions of free space radiation with the lunar crust; and, particles produced by decays of radioactive elements in the lunar crust.</obo:IAO_0000115>
        <rdfs:label>lunar surface radiation environment</rdfs:label>
    </owl:Class>
    


    <!-- http://purl.obolibrary.org/obo/SLSO_1100025 -->

    <owl:Class rdf:about="http://purl.obolibrary.org/obo/SLSO_1100025">
        <rdfs:subClassOf rdf:resource="http://purl.obolibrary.org/obo/SLSO_1100030"/>
        <obo:IAO_0000115>The natural radiation environment in Mars orbit. Contributions to the Mars orbit radiation environment include: free space radiation, partially shielded by the planetary body; albedo radiation produced by interactions of free space radiation with the Mars crust and modulated by interactions with the Martian atmosphere; and, particles produced by decays of radioactive elements in the Martian crust modulated by interactions with the Martian atmosphere.</obo:IAO_0000115>
        <rdfs:label>mars orbit radiation environment</rdfs:label>
    </owl:Class>
    


    <!-- http://purl.obolibrary.org/obo/SLSO_1100026 -->

    <owl:Class rdf:about="http://purl.obolibrary.org/obo/SLSO_1100026">
        <rdfs:subClassOf rdf:resource="http://purl.obolibrary.org/obo/SLSO_1100029"/>
        <rdfs:subClassOf rdf:resource="http://purl.obolibrary.org/obo/SLSO_1100030"/>
        <obo:IAO_0000115>The natural radiation environment on or adjacent to the surface of Mars. Contributions to the lunar surface radiation environment include: free space radiation partially shielded by the planetary body and modulated by interactions with the Martian atmosphere; albedo radiation produced by interactions of free space radiation with the Martian crust; and, particles produced by decays of radioactive elements in the Martian crust.</obo:IAO_0000115>
        <rdfs:label>mars surface radiation environment</rdfs:label>
    </owl:Class>
    


    <!-- http://purl.obolibrary.org/obo/SLSO_1100027 -->

    <owl:Class rdf:about="http://purl.obolibrary.org/obo/SLSO_1100027">
        <rdfs:subClassOf rdf:resource="http://purl.obolibrary.org/obo/SLSO_1100029"/>
        <obo:IAO_0000115>The natural radiation environment of a region of a planetary surface</obo:IAO_0000115>
        <rdfs:label>planet surface radiation environment</rdfs:label>
    </owl:Class>
    


    <!-- http://purl.obolibrary.org/obo/SLSO_1100029 -->

    <owl:Class rdf:about="http://purl.obolibrary.org/obo/SLSO_1100029">
        <rdfs:subClassOf rdf:resource="http://purl.obolibrary.org/obo/SLSO_1100019"/>
        <obo:IAO_0000115>The natural radiation environment on or adjacent to the surface of a planet or moon, comprising: the free space radiation environment partially shielded by the planet or moon and modulated by interactions with the planet&apos;s or moon&apos;s crust, and atmosphere and magnetic field, if any, and radiation produced by naturally occurring radioactive elements in the planet&apos;s or moon&apos;s crust. A surface radiation environment can include both ionizing radiation and non-ionizing radiation such as UVA, UVB and visible light, but often is used to refer to biologically damaging ionizing radiation such as galactic cosmic radiation and solar particles.</obo:IAO_0000115>
        <rdfs:label>surface radiation environment</rdfs:label>
    </owl:Class>
    


    <!-- http://purl.obolibrary.org/obo/SLSO_1100030 -->

    <owl:Class rdf:about="http://purl.obolibrary.org/obo/SLSO_1100030">
        <rdfs:subClassOf rdf:resource="http://purl.obolibrary.org/obo/SLSO_1100019"/>
        <obo:IAO_0000115>The natural radiation environment in the vicinity of Mars comprising: the free space radiation environment, radiation produced by interactions of the free space radiation environment with the Martian atmosphere and crust, and radiation produced by naturally occurring radioactive elements in the Martian crust. The Martian radiation environment varies with location and time--for example with proximity to the Martian surface, shielding by the planetary body, and with the solar cycle and periodic solar particle events. It can include both ionizing radiation and non-ionizing radiation such as UVA, UVB and visible light, but often is used to refer to biologically damaging ionizing radiation such as galactic cosmic radiation and solar particles.</obo:IAO_0000115>
        <oboInOwl:hasExactSynonym>martian radiation environment</oboInOwl:hasExactSynonym>
        <rdfs:label>mars radiation environment</rdfs:label>
    </owl:Class>
    


    <!-- http://purl.obolibrary.org/obo/SLSO_1100031 -->

    <owl:Class rdf:about="http://purl.obolibrary.org/obo/SLSO_1100031">
        <rdfs:subClassOf rdf:resource="http://purl.obolibrary.org/obo/SLSO_1100019"/>
        <obo:IAO_0000115>The natural radiation environment on or in the vicinity of the Earth&apos;s moon, comprising: the free space radiation environment, radiation produced by interactions of the free space radiation environment with the lunar surface, and radiation produced by naturally occurring radioactive elements in the lunar crust. The lunar radiation environment varies with location and time--for example with proximity to the lunar surface, shielding by the Moon itself, and with the solar cycle and periodic solar particle events. It can include both ionizing radiation and non-ionizing radiation such as UVA, UVB and visible light, but often is used to refer to biologically damaging ionizing radiation such as galactic cosmic radiation and solar particles.</obo:IAO_0000115>
        <rdfs:label>lunar radiation environment</rdfs:label>
    </owl:Class>
    


    <!-- http://purl.obolibrary.org/obo/SLSO_1100032 -->

    <owl:Class rdf:about="http://purl.obolibrary.org/obo/SLSO_1100032">
        <rdfs:subClassOf rdf:resource="http://purl.obolibrary.org/obo/SLSO_1100010"/>
        <rdfs:label>lunar orbit environment</rdfs:label>
    </owl:Class>
    


    <!-- http://purl.obolibrary.org/obo/SLSO_1100033 -->

    <owl:Class rdf:about="http://purl.obolibrary.org/obo/SLSO_1100033">
        <rdfs:subClassOf rdf:resource="http://purl.obolibrary.org/obo/SLSO_1100010"/>
        <rdfs:label>lunar surface environment</rdfs:label>
    </owl:Class>
    


    <!-- http://purl.obolibrary.org/obo/SLSO_1100034 -->

    <owl:Class rdf:about="http://purl.obolibrary.org/obo/SLSO_1100034">
        <rdfs:subClassOf rdf:resource="http://purl.obolibrary.org/obo/SLSO_1100010"/>
        <oboInOwl:hasExactSynonym>martian orbit environment</oboInOwl:hasExactSynonym>
        <rdfs:label>mars orbit environment</rdfs:label>
    </owl:Class>
    


    <!-- http://purl.obolibrary.org/obo/SLSO_1100035 -->

    <owl:Class rdf:about="http://purl.obolibrary.org/obo/SLSO_1100035">
        <rdfs:subClassOf rdf:resource="http://purl.obolibrary.org/obo/SLSO_1100010"/>
        <oboInOwl:hasExactSynonym>martian surface environment</oboInOwl:hasExactSynonym>
        <rdfs:label>mars surface environment</rdfs:label>
    </owl:Class>
    


    <!-- 
    ///////////////////////////////////////////////////////////////////////////////////////
    //
    // Individuals
    //
    ///////////////////////////////////////////////////////////////////////////////////////
     -->

    


    <!-- http://purl.obolibrary.org/obo/SLSO_1000000 -->

    <owl:NamedIndividual rdf:about="http://purl.obolibrary.org/obo/SLSO_1000000">
        <rdf:type rdf:resource="http://purl.obolibrary.org/obo/SLSO_0000051"/>
        <rdfs:label>International Space Station</rdfs:label>
    </owl:NamedIndividual>
    


    <!-- http://purl.obolibrary.org/obo/SLSO_1000001 -->

    <owl:NamedIndividual rdf:about="http://purl.obolibrary.org/obo/SLSO_1000001">
        <rdf:type rdf:resource="http://purl.obolibrary.org/obo/ENVO_00003919"/>
        <obo:IAO_0000115>An underwater habitat and research laboratory deployed on the ocean floor at a depth of 62 feet/19 meters and located 3.5 miles/6.5 km from Key Largo, FL.  The installation consists of a surface-level life support buoy, the 45ft/14m x 9.8ft/3m habitat with living quarters, life-support systems, and laboratory space, and two underwater waystations supplying air for aquanauts on extended dives outside the habitat.  The habitat includes a wet entry porch, a pressurizable main cabin, and a sealable entry lock connecting the two pressure zones.  Saturation diving allows crews of up to six people to conduct extended missions while living in the habitat.  Aquarius enables spaceflight analog studies approximating extreme space environments, extravehicular activity, and isolation and confinement of crew.  </obo:IAO_0000115>
        <rdfs:label>Aquarius</rdfs:label>
    </owl:NamedIndividual>
    <owl:Axiom>
        <owl:annotatedSource rdf:resource="http://purl.obolibrary.org/obo/SLSO_1000001"/>
        <owl:annotatedProperty rdf:resource="http://purl.obolibrary.org/obo/IAO_0000115"/>
        <owl:annotatedTarget>An underwater habitat and research laboratory deployed on the ocean floor at a depth of 62 feet/19 meters and located 3.5 miles/6.5 km from Key Largo, FL.  The installation consists of a surface-level life support buoy, the 45ft/14m x 9.8ft/3m habitat with living quarters, life-support systems, and laboratory space, and two underwater waystations supplying air for aquanauts on extended dives outside the habitat.  The habitat includes a wet entry porch, a pressurizable main cabin, and a sealable entry lock connecting the two pressure zones.  Saturation diving allows crews of up to six people to conduct extended missions while living in the habitat.  Aquarius enables spaceflight analog studies approximating extreme space environments, extravehicular activity, and isolation and confinement of crew.  </owl:annotatedTarget>
        <obo:IAO_0000119>References: Sandra H�uplik-Meusburger and Sheryl Bishop, Space Habitats and Habitability: Designing for Isolated and Confined Environments on Earth and in Space (Cham, Switzerland: Springer Nature Switzerland, 2021).  NASA NEEMO page:  [https://www.nasa.gov/mission/neemo/]</obo:IAO_0000119>
    </owl:Axiom>
    


    <!-- http://purl.obolibrary.org/obo/SLSO_1000002 -->

    <owl:NamedIndividual rdf:about="http://purl.obolibrary.org/obo/SLSO_1000002">
        <rdf:type rdf:resource="http://purl.obolibrary.org/obo/SLSO_0000051"/>
        <rdfs:label>Atlantis</rdfs:label>
    </owl:NamedIndividual>
    


    <!-- http://purl.obolibrary.org/obo/SLSO_1000003 -->

    <owl:NamedIndividual rdf:about="http://purl.obolibrary.org/obo/SLSO_1000003">
        <rdf:type rdf:resource="http://purl.obolibrary.org/obo/SLSO_0000051"/>
        <rdfs:label>Challenger</rdfs:label>
    </owl:NamedIndividual>
    


    <!-- http://purl.obolibrary.org/obo/SLSO_1000004 -->

    <owl:NamedIndividual rdf:about="http://purl.obolibrary.org/obo/SLSO_1000004">
        <rdf:type rdf:resource="http://purl.obolibrary.org/obo/SLSO_0000051"/>
        <rdfs:label>Columbia</rdfs:label>
    </owl:NamedIndividual>
    


    <!-- http://purl.obolibrary.org/obo/SLSO_1000005 -->

    <owl:NamedIndividual rdf:about="http://purl.obolibrary.org/obo/SLSO_1000005">
        <rdf:type rdf:resource="http://purl.obolibrary.org/obo/SLSO_0000051"/>
        <rdfs:label>Cygnus</rdfs:label>
    </owl:NamedIndividual>
    


    <!-- http://purl.obolibrary.org/obo/SLSO_1000006 -->

    <owl:NamedIndividual rdf:about="http://purl.obolibrary.org/obo/SLSO_1000006">
        <rdf:type rdf:resource="http://purl.obolibrary.org/obo/SLSO_0000051"/>
        <rdfs:label>Discovery</rdfs:label>
    </owl:NamedIndividual>
    


    <!-- http://purl.obolibrary.org/obo/SLSO_1000007 -->

    <owl:NamedIndividual rdf:about="http://purl.obolibrary.org/obo/SLSO_1000007">
        <rdf:type rdf:resource="http://purl.obolibrary.org/obo/SLSO_0000051"/>
        <rdfs:label>Dragon</rdfs:label>
    </owl:NamedIndividual>
    


    <!-- http://purl.obolibrary.org/obo/SLSO_1000008 -->

    <owl:NamedIndividual rdf:about="http://purl.obolibrary.org/obo/SLSO_1000008">
        <rdf:type rdf:resource="http://purl.obolibrary.org/obo/SLSO_0000051"/>
        <rdfs:label>Endeavour</rdfs:label>
    </owl:NamedIndividual>
    


    <!-- http://purl.obolibrary.org/obo/SLSO_1000009 -->

    <owl:NamedIndividual rdf:about="http://purl.obolibrary.org/obo/SLSO_1000009">
        <rdf:type rdf:resource="http://purl.obolibrary.org/obo/SLSO_0000051"/>
        <rdfs:label>Foton-M2</rdfs:label>
    </owl:NamedIndividual>
    


    <!-- http://purl.obolibrary.org/obo/SLSO_1000010 -->

    <owl:NamedIndividual rdf:about="http://purl.obolibrary.org/obo/SLSO_1000010">
        <rdf:type rdf:resource="http://purl.obolibrary.org/obo/SLSO_0000051"/>
        <rdfs:label>Foton-M3</rdfs:label>
    </owl:NamedIndividual>
    


    <!-- http://purl.obolibrary.org/obo/SLSO_1000011 -->

    <owl:NamedIndividual rdf:about="http://purl.obolibrary.org/obo/SLSO_1000011">
        <rdf:type rdf:resource="http://purl.obolibrary.org/obo/SLSO_0000051"/>
        <rdfs:label>Mercury-Atlas 5</rdfs:label>
    </owl:NamedIndividual>
    


    <!-- http://purl.obolibrary.org/obo/SLSO_1000012 -->

    <owl:NamedIndividual rdf:about="http://purl.obolibrary.org/obo/SLSO_1000012">
        <rdf:type rdf:resource="http://purl.obolibrary.org/obo/SLSO_0000051"/>
        <rdfs:label>Mercury-Atlas 6</rdfs:label>
    </owl:NamedIndividual>
    


    <!-- http://purl.obolibrary.org/obo/SLSO_1000013 -->

    <owl:NamedIndividual rdf:about="http://purl.obolibrary.org/obo/SLSO_1000013">
        <rdf:type rdf:resource="http://purl.obolibrary.org/obo/SLSO_0000051"/>
        <rdfs:label>Mercury-Atlas 7</rdfs:label>
    </owl:NamedIndividual>
    


    <!-- http://purl.obolibrary.org/obo/SLSO_1000014 -->

    <owl:NamedIndividual rdf:about="http://purl.obolibrary.org/obo/SLSO_1000014">
        <rdf:type rdf:resource="http://purl.obolibrary.org/obo/SLSO_0000051"/>
        <rdfs:label>Mercury-Atlas 8</rdfs:label>
    </owl:NamedIndividual>
    


    <!-- http://purl.obolibrary.org/obo/SLSO_1000015 -->

    <owl:NamedIndividual rdf:about="http://purl.obolibrary.org/obo/SLSO_1000015">
        <rdf:type rdf:resource="http://purl.obolibrary.org/obo/SLSO_0000051"/>
        <rdfs:label>Mercury-Atlas 9</rdfs:label>
    </owl:NamedIndividual>
    


    <!-- http://purl.obolibrary.org/obo/SLSO_1000016 -->

    <owl:NamedIndividual rdf:about="http://purl.obolibrary.org/obo/SLSO_1000016">
        <rdf:type rdf:resource="http://purl.obolibrary.org/obo/SLSO_0000051"/>
        <rdfs:label>Mercury-Redstone 2</rdfs:label>
    </owl:NamedIndividual>
    


    <!-- http://purl.obolibrary.org/obo/SLSO_1000017 -->

    <owl:NamedIndividual rdf:about="http://purl.obolibrary.org/obo/SLSO_1000017">
        <rdf:type rdf:resource="http://purl.obolibrary.org/obo/SLSO_0000051"/>
        <rdfs:label>Mercury-Redstone 3</rdfs:label>
    </owl:NamedIndividual>
    


    <!-- http://purl.obolibrary.org/obo/SLSO_1000018 -->

    <owl:NamedIndividual rdf:about="http://purl.obolibrary.org/obo/SLSO_1000018">
        <rdf:type rdf:resource="http://purl.obolibrary.org/obo/SLSO_0000051"/>
        <rdfs:label>Mercury-Redstone 4</rdfs:label>
    </owl:NamedIndividual>
    


    <!-- http://purl.obolibrary.org/obo/SLSO_1000019 -->

    <owl:NamedIndividual rdf:about="http://purl.obolibrary.org/obo/SLSO_1000019">
        <rdf:type rdf:resource="http://purl.obolibrary.org/obo/SLSO_0000051"/>
        <rdfs:label>Minotaur IV</rdfs:label>
    </owl:NamedIndividual>
    


    <!-- http://purl.obolibrary.org/obo/SLSO_1000020 -->

    <owl:NamedIndividual rdf:about="http://purl.obolibrary.org/obo/SLSO_1000020">
        <rdf:type rdf:resource="http://purl.obolibrary.org/obo/SLSO_0000051"/>
        <rdfs:label>Mir Space Station</rdfs:label>
    </owl:NamedIndividual>
    


    <!-- http://purl.obolibrary.org/obo/SLSO_1000021 -->

    <owl:NamedIndividual rdf:about="http://purl.obolibrary.org/obo/SLSO_1000021">
        <rdf:type rdf:resource="http://purl.obolibrary.org/obo/SLSO_0000051"/>
        <rdfs:label>Saturn 1B</rdfs:label>
    </owl:NamedIndividual>
    


    <!-- http://purl.obolibrary.org/obo/SLSO_1000022 -->

    <owl:NamedIndividual rdf:about="http://purl.obolibrary.org/obo/SLSO_1000022">
        <rdf:type rdf:resource="http://purl.obolibrary.org/obo/SLSO_0000051"/>
        <rdfs:label>Saturn V</rdfs:label>
    </owl:NamedIndividual>
    


    <!-- http://purl.obolibrary.org/obo/SLSO_1000023 -->

    <owl:NamedIndividual rdf:about="http://purl.obolibrary.org/obo/SLSO_1000023">
        <rdf:type rdf:resource="http://purl.obolibrary.org/obo/SLSO_0000051"/>
        <rdfs:label>Scout Satellite</rdfs:label>
    </owl:NamedIndividual>
    


    <!-- http://purl.obolibrary.org/obo/SLSO_1000024 -->

    <owl:NamedIndividual rdf:about="http://purl.obolibrary.org/obo/SLSO_1000024">
        <rdf:type rdf:resource="http://purl.obolibrary.org/obo/SLSO_0000051"/>
        <rdfs:label>Shuttle</rdfs:label>
    </owl:NamedIndividual>
    


    <!-- http://purl.obolibrary.org/obo/SLSO_1000025 -->

    <owl:NamedIndividual rdf:about="http://purl.obolibrary.org/obo/SLSO_1000025">
        <rdf:type rdf:resource="http://purl.obolibrary.org/obo/SLSO_0000051"/>
        <rdfs:label>Soyuz</rdfs:label>
    </owl:NamedIndividual>
    


    <!-- http://purl.obolibrary.org/obo/SLSO_1000026 -->

    <owl:NamedIndividual rdf:about="http://purl.obolibrary.org/obo/SLSO_1000026">
        <rdf:type rdf:resource="http://purl.obolibrary.org/obo/SLSO_0000051"/>
        <rdfs:label>Thor Delta</rdfs:label>
    </owl:NamedIndividual>
    


    <!-- http://purl.obolibrary.org/obo/SLSO_1000027 -->

    <owl:NamedIndividual rdf:about="http://purl.obolibrary.org/obo/SLSO_1000027">
        <rdf:type rdf:resource="http://purl.obolibrary.org/obo/SLSO_0000051"/>
        <rdfs:label>Titan II</rdfs:label>
    </owl:NamedIndividual>
    


    <!-- http://purl.obolibrary.org/obo/SLSO_1000028 -->

    <owl:NamedIndividual rdf:about="http://purl.obolibrary.org/obo/SLSO_1000028">
        <rdf:type rdf:resource="http://purl.obolibrary.org/obo/SLSO_0000051"/>
        <rdfs:label>Vostok</rdfs:label>
    </owl:NamedIndividual>
    


    <!-- http://purl.obolibrary.org/obo/SLSO_1000029 -->

    <owl:NamedIndividual rdf:about="http://purl.obolibrary.org/obo/SLSO_1000029">
        <rdf:type rdf:resource="http://purl.obolibrary.org/obo/SLSO_0000051"/>
        <rdfs:label>Vostok (modified)</rdfs:label>
    </owl:NamedIndividual>
    


    <!-- http://purl.obolibrary.org/obo/SLSO_1100000 -->

    <owl:NamedIndividual rdf:about="http://purl.obolibrary.org/obo/SLSO_1100000">
        <rdf:type rdf:resource="http://purl.obolibrary.org/obo/ENVO_00000469"/>
        <rdfs:label>Mars 500 Chamber</rdfs:label>
    </owl:NamedIndividual>
    


    <!-- http://purl.obolibrary.org/obo/SLSO_1100001 -->

    <owl:NamedIndividual rdf:about="http://purl.obolibrary.org/obo/SLSO_1100001">
        <rdf:type rdf:resource="http://purl.obolibrary.org/obo/ENVO_00000469"/>
        <rdfs:label>MEDES Space Clinic</rdfs:label>
    </owl:NamedIndividual>
    


    <!-- http://purl.obolibrary.org/obo/SLSO_1100002 -->

    <owl:NamedIndividual rdf:about="http://purl.obolibrary.org/obo/SLSO_1100002">
        <rdf:type rdf:resource="http://purl.obolibrary.org/obo/ENVO_00000469"/>
        <rdfs:label>NASA Ames Research Center (ARC)</rdfs:label>
    </owl:NamedIndividual>
    


    <!-- http://purl.obolibrary.org/obo/SLSO_1100003 -->

    <owl:NamedIndividual rdf:about="http://purl.obolibrary.org/obo/SLSO_1100003">
        <rdf:type rdf:resource="http://purl.obolibrary.org/obo/ENVO_00000469"/>
        <rdfs:label>NASA Johnson Space Center (JSC)</rdfs:label>
    </owl:NamedIndividual>
    


    <!-- http://purl.obolibrary.org/obo/SLSO_1100004 -->

    <owl:NamedIndividual rdf:about="http://purl.obolibrary.org/obo/SLSO_1100004">
        <rdf:type rdf:resource="http://purl.obolibrary.org/obo/ENVO_00000469"/>
        <rdfs:label>Variable Pressure Chamber</rdfs:label>
    </owl:NamedIndividual>
    


    <!-- http://purl.obolibrary.org/obo/SLSO_1100005 -->

    <owl:NamedIndividual rdf:about="http://purl.obolibrary.org/obo/SLSO_1100005">
        <rdf:type rdf:resource="http://purl.obolibrary.org/obo/ENVO_00000469"/>
        <rdfs:label>UTMB FARU</rdfs:label>
    </owl:NamedIndividual>
    


    <!-- http://purl.obolibrary.org/obo/SLSO_1100006 -->

    <owl:NamedIndividual rdf:about="http://purl.obolibrary.org/obo/SLSO_1100006">
        <rdf:type rdf:resource="http://purl.obolibrary.org/obo/ENVO_00000469"/>
        <rdfs:label>UTMB GCRC</rdfs:label>
    </owl:NamedIndividual>
    


    <!-- http://purl.obolibrary.org/obo/SLSO_1100007 -->

    <owl:NamedIndividual rdf:about="http://purl.obolibrary.org/obo/SLSO_1100007">
        <rdf:type rdf:resource="http://purl.obolibrary.org/obo/ENVO_00000469"/>
        <obo:IAO_0000115>The NEK facility is located at the Institute of Biomedical Problems (IBMP) at the Russian Academy of Sciences in Moscow, Russia. It is a multi-compartment, pressurized facility that is used to capture subjects&apos; emotional and mental state in long-duration isolated and confined environment to advance understanding of behavioral risks associated with this type of spaceflight analog. Subjects are physically isolated and have limited communication to the outside world. This enables subjects to feel as if they are in an actual spaceflight environment. The two areas of study are behavioral health and biochemistry, which will monitor subjects� psychological health and cortisol levels, respectively.</obo:IAO_0000115>
        <rdfs:label>NEK</rdfs:label>
    </owl:NamedIndividual>
    


    <!-- http://purl.obolibrary.org/obo/SLSO_1100008 -->

    <owl:NamedIndividual rdf:about="http://purl.obolibrary.org/obo/SLSO_1100008">
        <rdf:type rdf:resource="http://purl.obolibrary.org/obo/ENVO_00000469"/>
        <obo:IAO_0000115>:envihab is a state-of-the-art research facility located in Cologne, Germany.</obo:IAO_0000115>
        <rdfs:label>envihab</rdfs:label>
    </owl:NamedIndividual>
    


    <!-- http://purl.obolibrary.org/obo/SLSO_1100009 -->

    <owl:NamedIndividual rdf:about="http://purl.obolibrary.org/obo/SLSO_1100009">
        <rdf:type rdf:resource="http://purl.obolibrary.org/obo/ENVO_00000469"/>
        <obo:IAO_0000115>The HERA facility is located at the Johnson Space Center in Houston, Texas and consists of a unique three-story closed habitat that is designed to serve as an analog for isolation, confinement, and remote conditions in exploration scenarios. Subjects� emotional and mental states in a short-duration, isolated, and confined environment are captured to advance understanding of behavioral risks associated with this type of spaceflight analog. The two areas of study are behavioral health and biochemistry, which monitor subjects� psychological health and cortisol levels, respectively. </obo:IAO_0000115>
        <rdfs:label>HERA</rdfs:label>
    </owl:NamedIndividual>
</rdf:RDF>



<!-- Generated by the OWL API (version 4.5.29) https://github.com/owlcs/owlapi -->

